Correct proofs for `Imppair`.

casestudy/imp/Imppairs.v
@@ -1,11 +1,10 @@
 (* Imp with pairs *)
-(* TODO: the eval inductive type *)
 family Imppairs extends Impzero { }
 
 family Imppairs.Impcommon {                 
   Inductive expression : Type +=
-     | Epair : expr -> expr -> expr.  
-}  
+     | Epair : expression -> expression -> expression.  
+}
 
 family Imppairs.Impcommon {
     family Semantics.Values {
@@ -16,6 +15,32 @@ family Imppairs.Impcommon {
 
 family Imppairs.Impcommon {
   family Semantics {
-      
-  }    
-}    
+      Inductive eval_expr : expression -> Values.value -> Prop :=
+          | eval_Epair : forall e1 e2 v1 v2,
+            eval_expr e1 v1 ->
+            eval_expr e2 v2 ->
+            eval_epxr (Epair e1 e2) (Vpair v1 v2)
+  }
+}
+
+family Imppairs.Impgen {
+  Fixpoint translate_expression :=
+    Case Epair := ...
+                  
+  family Proofs {
+       Lemma translate_expression_correct:
+           forall a v,
+           [self].Source.Semantics.eval_expr a v ->
+           forall ta, translate_expression a = OK ta ->
+           [self].Target.Semantics.eval_expr ta v.
+       Proof.
+         Case Epair := ...
+       Qed.
+  }
+}  
+
+(* Inherited from Impgen *)
+family Imppairs.Impshmgen { }
+
+(* Inherited from Impgen *)                          
+family Imppairs.Impminorgen { }      
